src/KT/KT_defs.lean
@@ -1,0 +1,61 @@
+import defs
+open nnf
+
+structure seqt : Type :=
+(main : list nnf)
+(hdld : list nnf) -- handled boxes
+
+structure KT (states : Type) extends kripke states :=
+(refl  : reflexive rel)
+
+instance inhabited_KT : inhabited (KT ℕ) := 
+⟨{ val := λ a b, tt, rel := λ a b, tt, refl := λ a, by simp }⟩
+
+@[simp] def force {states : Type} (k : KT states) : states → nnf → Prop
+| s (var n)    := k.val n s
+| s (neg n)    := ¬ k.val n s
+| s (and φ ψ)  := force s φ ∧ force s ψ
+| s (or φ ψ)   := force s φ ∨ force s ψ
+| s (box φ)    := ∀ s', k.rel s s' → force s' φ
+| s (dia φ)    := ∃ s', k.rel s s' ∧ force s' φ
+
+def sat {st} (k : KT st) (s) (Γ : list nnf) : Prop := 
+∀ φ ∈ Γ, force k s φ
+
+def unsatisfiable (Γ : list nnf) : Prop := 
+∀ (st) (k : KT st) s, ¬ sat k s Γ
+
+theorem unsat_singleton {φ} : unsatisfiable [φ] → ∀ (st) (k : KT st) s, ¬ force k s φ
+ := 
+begin
+  intro h, intros, intro hf, 
+  apply h, intros ψ hψ, rw list.mem_singleton at hψ, rw hψ, exact hf
+end
+
+theorem sat_of_empty {st} (k : KT st) (s) : sat k s [] :=
+λ φ h, absurd h $ list.not_mem_nil _
+
+theorem ne_empty_of_unsat {Γ} (h : unsatisfiable Γ): Γ ≠ [] := 
+begin 
+  intro heq, rw heq at h, 
+  apply h, apply sat_of_empty, exact nat, 
+  apply inhabited_KT.1, exact 0 
+end
+
+class val_constructible (Γ : seqt) :=
+(satu : saturated Γ.main)
+(no_box_main : ∀ {φ}, box φ ∉ Γ.main)
+(no_contra_main : ∀ {n}, var n ∈ Γ.main → neg n ∉ Γ.main)
+(v : list ℕ)
+(hv : ∀ n, var n ∈ Γ.main ↔ n ∈ v)
+
+class modal_applicable (Γ : seqt) extends val_constructible Γ :=
+(φ : nnf)
+(ex : dia φ ∈ Γ.main)
+
+class model_constructible (Γ : seqt) extends val_constructible Γ :=
+(no_dia : ∀ {φ}, nnf.dia φ ∉ Γ.main)
+
+inductive and_instance_seqt (Γ : seqt) : seqt → Type
+| cons : Π {φ ψ}, nnf.and φ ψ ∈ Γ.main → 
+         and_instance_seqt ⟨φ :: ψ :: Γ.main.erase (and φ ψ), Γ.hdld⟩
