src/KT/rules.lean
@@ -7,4 +7,26 @@ open nnf subtype list
 
 inductive node (Γ : seqt) : Type
 | closed : unsatisfiable (Γ.main ++ Γ.hdld) → node
--- | open_ : {s // sat }
+| open_ : {s // sat builder s (Γ.main ++ Γ.hdld)} → node
+
+open node
+
+def contra_rule_seqt {Δ : seqt} {n} (h : var n ∈ Δ.main ∧ neg n ∈ Δ.main) : node Δ := 
+begin
+  left,
+  {exact unsat_contra_seqt h.1 h.2}
+end
+
+def and_rule_seqt {Γ Δ : seqt} (i : and_instance_seqt Γ Δ) : node Δ → node Γ
+| (closed h) := begin 
+                      left, 
+                      {apply unsat_of_closed_and, repeat {assumption}}, 
+                    end
+
+| (open_ w)  := begin
+                  right,
+                  clear and_rule,
+                  cases i with φ ψ h,
+                  constructor,
+                  exact sat_and_of_sat_split _ _ _ _ _ h w.2
+                end
